Some clean up/tweaks of locks.

heap_lang/lib/lock.v
@@ -1,32 +1,29 @@
-(** Abstract Lock Interface **)
-
 From iris.heap_lang Require Import heap notation.
 
-Structure lock Σ `{!heapG Σ} :=
-  Lock {
-      (* -- operations -- *)
-      newlock : val;
-      acquire : val;
-      release : val;
-      (* -- predicates -- *)
-      (* name is used to associate locked with is_lock *)
-      name: Type;
-      is_lock (N: namespace) (γ: name) (lock: val) (R: iProp Σ) : iProp Σ;
-      locked (γ: name) : iProp Σ;
-      (* -- general properties -- *)
-      is_lock_ne N γ lk n: Proper (dist n ==> dist n) (is_lock N γ lk);
-      is_lock_persistent N γ lk R : PersistentP (is_lock N γ lk R);
-      locked_timeless γ : TimelessP (locked γ);
-      locked_exclusive γ : locked γ ★ locked γ ⊢ False;
-      (* -- operation specs -- *)
-      newlock_spec N (R : iProp Σ) Φ :
-        heapN ⊥ N →
-        heap_ctx ★ R ★ (∀ l γ, is_lock N γ l R -★ Φ l) ⊢ WP newlock #() {{ Φ }};
-      acquire_spec N γ lk R (Φ : val → iProp Σ) :
-        is_lock N γ lk R ★ (locked γ -★ R -★ Φ #()) ⊢ WP acquire lk {{ Φ }};
-      release_spec N γ lk R (Φ : val → iProp Σ) :
-        is_lock N γ lk R ★ locked γ ★ R ★ Φ #() ⊢ WP release lk {{ Φ }}
-    }.
+Structure lock Σ `{!heapG Σ} := Lock {
+  (* -- operations -- *)
+  newlock : val;
+  acquire : val;
+  release : val;
+  (* -- predicates -- *)
+  (* name is used to associate locked with is_lock *)
+  name : Type;
+  is_lock (N: namespace) (γ: name) (lock: val) (R: iProp Σ) : iProp Σ;
+  locked (γ: name) : iProp Σ;
+  (* -- general properties -- *)
+  is_lock_ne N γ lk n: Proper (dist n ==> dist n) (is_lock N γ lk);
+  is_lock_persistent N γ lk R : PersistentP (is_lock N γ lk R);
+  locked_timeless γ : TimelessP (locked γ);
+  locked_exclusive γ : locked γ ★ locked γ ⊢ False;
+  (* -- operation specs -- *)
+  newlock_spec N (R : iProp Σ) Φ :
+    heapN ⊥ N →
+    heap_ctx ★ R ★ (∀ l γ, is_lock N γ l R -★ Φ l) ⊢ WP newlock #() {{ Φ }};
+  acquire_spec N γ lk R (Φ : val → iProp Σ) :
+    is_lock N γ lk R ★ (locked γ -★ R -★ Φ #()) ⊢ WP acquire lk {{ Φ }};
+  release_spec N γ lk R (Φ : val → iProp Σ) :
+    is_lock N γ lk R ★ locked γ ★ R ★ Φ #() ⊢ WP release lk {{ Φ }}
+}.
 
 Arguments newlock {_ _} _.
 Arguments acquire {_ _} _.
